<?xml version="1.0"?>


<!DOCTYPE rdf:RDF [
    <!ENTITY owl "http://www.w3.org/2002/07/owl#" >
    <!ENTITY xsd "http://www.w3.org/2001/XMLSchema#" >
    <!ENTITY rdfs "http://www.w3.org/2000/01/rdf-schema#" >
    <!ENTITY rdf "http://www.w3.org/1999/02/22-rdf-syntax-ns#" >
]>


<rdf:RDF xmlns="http://purl.org/emmedi/hico#"
     xml:base="http://purl.org/emmedi/hico"
     xmlns:rdfs="http://www.w3.org/2000/01/rdf-schema#"
     xmlns:owl="http://www.w3.org/2002/07/owl#"
     xmlns:xsd="http://www.w3.org/2001/XMLSchema#"
     xmlns:rdf="http://www.w3.org/1999/02/22-rdf-syntax-ns#">
    <owl:Ontology rdf:about="http://purl.org/emmedi/hico">
        <rdfs:label xml:lang="en">The Historical Context Ontology (HiCO)</rdfs:label>
        <rdfs:comment xml:lang="en">The Historical Context Ontology (HiCO) is an OWL 2 DL ontology developed for representing the context of a claim. In particular, it addresses features characterising hermeneutical activities performed by scholars while generating new information (i.e. an interpretation act). It allows to represent and reason on reliability of argumentations around attributions, by evaluating features such as motivations, types of cited sources or criteria, dates, relations with other claims (e.g. agreement/disagreement). Specifically, historical context regards events and situations that are part of the life-cycle of cultural heritage objects. For instance, &quot;being created by somebody&quot;, or &quot;being created at a certain time&quot;, are events related to an artefact that are claimed by an agent at a certain time, motivated with usage of primary sources, and recorded in a secondary source (e.g. a cataloguing record).
            
HiCO extends the PROV Ontology (http://www.w3.org/ns/prov) with terms for describing aspects of the hermeneutical activity, and reuses existing ontologies, such as CiTO Ontology (http://purl.org/spar/cito/) for linking attributions to related sources.</rdfs:comment>
    </owl:Ontology>
    


    <!-- 
    ///////////////////////////////////////////////////////////////////////////////////////
    //
    // Object Properties
    //
    ///////////////////////////////////////////////////////////////////////////////////////
     -->

    


    <!-- http://purl.org/emmedi/hico/hasInterpretationCriterion -->

    <owl:ObjectProperty rdf:about="http://purl.org/emmedi/hico/hasInterpretationCriterion">
        <rdfs:label xml:lang="en">has interpretation criterion</rdfs:label>
        <rdfs:comment xml:lang="en">A property relating an interpretation act to a criterion or type of source used to support the claim.</rdfs:comment>
        <rdfs:isDefinedBy rdf:resource="http://purl.org/emmedi/hico"/>
        <rdfs:domain rdf:resource="http://purl.org/emmedi/hico/InterpretationAct"/>
        <rdfs:range rdf:resource="http://purl.org/emmedi/hico/InterpretationCriterion"/>
    </owl:ObjectProperty>
    


    <!-- http://purl.org/emmedi/hico/hasInterpretationType -->

    <owl:ObjectProperty rdf:about="http://purl.org/emmedi/hico/hasInterpretationType">
        <rdfs:label xml:lang="en">has interpretation type</rdfs:label>
        <rdfs:comment xml:lang="en">A property relating an interpretation act to an individual defining an arbitrary classification of the interpretation.</rdfs:comment>
        <rdfs:isDefinedBy rdf:resource="http://purl.org/emmedi/hico"/>
        <rdfs:domain rdf:resource="http://purl.org/emmedi/hico/InterpretationAct"/>
        <rdfs:range rdf:resource="http://purl.org/emmedi/hico/InterpretationType"/>
    </owl:ObjectProperty>
    


    <!-- http://purl.org/emmedi/hico/isExtractedFrom -->

    <owl:ObjectProperty rdf:about="http://purl.org/emmedi/hico/isExtractedFrom">
        <rdfs:label xml:lang="en">is extracted from</rdfs:label>
        <rdfs:comment xml:lang="en">A property relating an interpretation act to the source where from the claim has been extracted.</rdfs:comment>
        <rdfs:isDefinedBy rdf:resource="http://purl.org/emmedi/hico"/>
        <rdfs:domain rdf:resource="http://purl.org/emmedi/hico/InterpretationAct"/>
        <rdfs:subPropertyOf rdf:resource="http://www.w3.org/ns/prov#wasInfluencedBy"/>
    </owl:ObjectProperty>
    


    <!-- http://purl.org/spar/cito/agreesWith -->

    <owl:ObjectProperty rdf:about="http://purl.org/spar/cito/agreesWith">
        <rdfs:label xml:lang="en">agrees with</rdfs:label>
        <rdfs:isDefinedBy rdf:resource="http://purl.org/spar/cito"/>
    </owl:ObjectProperty>
    


    <!-- http://purl.org/spar/cito/citesAsEvidence -->

    <owl:ObjectProperty rdf:about="http://purl.org/spar/cito/citesAsEvidence">
        <rdfs:label xml:lang="en">cites as evidence</rdfs:label>
        <rdfs:isDefinedBy rdf:resource="http://purl.org/spar/cito"/>
    </owl:ObjectProperty>
    


    <!-- http://purl.org/spar/cito/disagreesWith -->

    <owl:ObjectProperty rdf:about="http://purl.org/spar/cito/disagreesWith">
        <rdfs:label xml:lang="en">disagrees with</rdfs:label>
        <rdfs:isDefinedBy rdf:resource="http://purl.org/spar/cito"/>
    </owl:ObjectProperty>
    


    <!-- http://purl.org/spar/cito/refutes -->

    <owl:ObjectProperty rdf:about="http://purl.org/spar/cito/refutes">
        <rdfs:label xml:lang="en">refutes</rdfs:label>
        <rdfs:isDefinedBy rdf:resource="http://purl.org/spar/cito"/>
    </owl:ObjectProperty>
    


    <!-- http://www.w3.org/TR/prov-o/#wasGeneratedBy -->

    <owl:ObjectProperty rdf:about="http://www.w3.org/TR/prov-o/#wasGeneratedBy">
        <rdfs:label xml:lang="en">was generated by</rdfs:label>
        <rdfs:comment xml:lang="en">A property relating statements to an interpretation act.</rdfs:comment>
        <rdfs:isDefinedBy rdf:resource="http://www.w3.org/ns/prov"/>
    </owl:ObjectProperty>
    


    <!-- http://www.w3.org/ns/prov#wasInfluencedBy -->

    <owl:ObjectProperty rdf:about="http://www.w3.org/ns/prov#wasInfluencedBy">
        <rdfs:label xml:lang="en">was influenced by</rdfs:label>
        <rdfs:isDefinedBy rdf:resource="http://www.w3.org/ns/prov"/>
    </owl:ObjectProperty>
    


    <!-- 
    ///////////////////////////////////////////////////////////////////////////////////////
    //
    // Data properties
    //
    ///////////////////////////////////////////////////////////////////////////////////////
     -->

    


    <!-- http://www.w3.org/ns/prov#startedAtTime -->

    <owl:DatatypeProperty rdf:about="http://www.w3.org/ns/prov#startedAtTime">
        <rdfs:label xml:lang="en">started at time</rdfs:label>
        <rdfs:comment xml:lang="en">A property relating an interpretation act to the time that triggered the activity.</rdfs:comment>
        <rdfs:isDefinedBy rdf:resource="http://www.w3.org/ns/prov"/>
    </owl:DatatypeProperty>
    


    <!-- 
    ///////////////////////////////////////////////////////////////////////////////////////
    //
    // Classes
    //
    ///////////////////////////////////////////////////////////////////////////////////////
     -->

    


    <!-- http://purl.org/emmedi/hico/InterpretationAct -->

    <owl:Class rdf:about="http://purl.org/emmedi/hico/InterpretationAct">
        <rdfs:label xml:lang="en">Interpretation Act</rdfs:label>
        <rdfs:subClassOf rdf:resource="http://www.w3.org/ns/prov#Activity"/>
        <rdfs:comment xml:lang="en">The hermeneutical activity performed by an agent in order to generate new information (e.g. an artwork attribution).</rdfs:comment>
        <rdfs:isDefinedBy rdf:resource="http://purl.org/emmedi/hico"/>
    </owl:Class>
    


    <!-- http://purl.org/emmedi/hico/InterpretationCriterion -->

    <owl:Class rdf:about="http://purl.org/emmedi/hico/InterpretationCriterion">
        <rdfs:label xml:lang="en">Interpretation Criterion</rdfs:label>
        <rdfs:comment xml:lang="en">The criterion or type of source used by an agent to support an interpretation act, such as bibliography, verbal communication, etc. </rdfs:comment>
        <rdfs:isDefinedBy rdf:resource="http://purl.org/emmedi/hico"/>
    </owl:Class>
    


    <!-- http://purl.org/emmedi/hico/InterpretationType -->

    <owl:Class rdf:about="http://purl.org/emmedi/hico/InterpretationType">
        <rdfs:label xml:lang="en">Interpretation Type</rdfs:label>
        <rdfs:comment xml:lang="en">An arbitrary definition of the interpretation act, such as artowork attribution or date attribution.</rdfs:comment>
        <rdfs:isDefinedBy rdf:resource="http://purl.org/emmedi/hico"/>
    </owl:Class>
    


    <!-- http://www.w3.org/ns/prov#Activity -->

    <owl:Class rdf:about="http://www.w3.org/ns/prov#Activity">
        <rdfs:label xml:lang="en">Activity</rdfs:label>
        <rdfs:isDefinedBy rdf:resource="http://www.w3.org/ns/prov"/>
    </owl:Class>
</rdf:RDF>



<!-- Generated by the OWL API (version 3.4.2) http://owlapi.sourceforge.net -->

